notary proofs

Notary.v
@@ -26,8 +26,14 @@ Section Notary.
   Theorem In_Nodes :
     forall (n : Name), (In n all_nodes).
   Proof.
-    destruct n ; auto.
-  Qed.
+    destruct n; [left|right;left]; auto.
+   Qed.
+
+  Theorem NoDup_Nodes : NoDup all_nodes.
+  Proof.
+    repeat constructor; auto.
+    intro. destruct H. discriminate. destruct H.
+   Qed. 
 
   Global Instance Notary_BaseParams : BaseParams :=
     {
@@ -36,21 +42,86 @@ Section Notary.
       output := string
     }.
 
+  Definition magic : string := "magic".
+  Definition staple s : string := magic ++ s.
+  Definition Handler (node _:Name) (msg:string) (_:Data)
+    : (list string * Data * list (Name * string) * list (@cryptoEvent Name))
+    :=
+    match node with
+    | Notary => ([],   tt, [], [Sign (staple msg)])
+    | Client => ([msg], tt, [], [Verify Notary msg])
+  end.
+  Definition inputHandler (_:Name) (_:unit) (d:Data)
+    : (list string * Data * list (Name * string) * list (@cryptoEvent Name))
+    := ([], d, [], [])
+  .
+
   Global Instance Notary_MultiParams : MultiParams Notary_BaseParams :=
     {
       name := Name ;
       msg  := string ;
       msg_eq_dec := string_dec ;
       name_eq_dec := Name_eq_dec ;
-      nodes :=  ;
-      all_names_nodes := In_n_Nodes ;
-      no_dup_nodes := nodup ;
+      nodes := all_nodes;
+      all_names_nodes := In_Nodes ;
+      no_dup_nodes := NoDup_Nodes ;
       init_handlers := init_data ;
-      net_handlers := fun dst src msg s =>
-                        runGenHandler_ignore s (NetHandler dst src msg) ;
-      input_handlers := fun nm msg s =>
-                          runGenHandler_ignore s (InputHandler nm msg)
+      net_handlers := Handler;
+      input_handlers := inputHandler
     }.
 
+  Definition magical s := exists t, s=staple t.
+  Lemma magical_staple : forall s, magical (staple s).
+    intros; unfold magical, staple. exists s.
+  Qed.
+
+  Lemma signed_magic : forall st trace,
+    refl_trans_n1_trace step_m step_m_init st trace ->
+    forall n s, In (n, Sign s) (nwCrypto st) -> magical s.
+    intros until 1.
+    remember step_m_init as s0 in H.
+    induction H; [subst; unfold step_m_init; simpl; intros; exfalso; auto|].
+    inversion H0; subst net net'. {
+      unfold net_handlers in *; simpl in *.
+      case_eq (pDst p); intro e; rewrite e in *; simpl in *. {
+        injection H1; clear H1; intros until n; revert n; subst; simpl in *.
+        intros.
+        destruct H1.
+        - injection H1; clear H1; intros; subst. apply magical_staple.
+        - eapply IHrefl_trans_n1_trace; eauto.
+      } {
+        injection H1; clear H1; intros; subst.
+        unfold mark_cevents_src in *; simpl in *. 
+        destruct H8; [discriminate|]; eauto.
+      }
+    } {
+      injection H1; clear H1; intros; subst; eauto.
+    }
+  Qed.
+
+  Goal forall st trace, step_m_star step_m_init st trace ->
+    forall (n:Name) (ss:list string), In (n, inr ss) trace ->
+    forall s, In s ss -> magical s.
+  Proof.
+    intros.
+    unfold step_m_star in *.
+    specialize (refl_trans_1n_n1_trace H); clear H; intro H.
+    remember step_m_init as s0 in H.
+    induction H; [inversion H0|]; rewrite Heqs0 in *; clear Heqs0.
+    destruct (in_app_or _ _ _ H0); try eauto.
+    inversion H2. {
+      unfold net_handlers in *; simpl in *.
+      case_eq (pDst p); intro e; rewrite e in *; clear e; simpl in *; 
+        injection H4; clear H4; intros; subst; simpl in *;
+        destruct H3; intuition; 
+        injection H3; clear H3; intros; subst; simpl in *; [exfalso; auto|].
+      eapply signed_magic; [eauto|].
+      edestruct H6; [left;eauto|discriminate|].
+      replace s with (pBody p) by intuition; eapply H3.
+   } { 
+    unfold net_handlers in *; subst; simpl in *.
+    destruct H3; intuition; discriminate.
+   }
+  Qed.
 
 End Notary.
